{-# OPTIONS --without-K --rewriting --termination-depth=2 #-}

{--- IMPORTANT! This version switches off termination checking temporarily. ---}

open import reedy.SimpleSemicategories
open import cwfs.CwFs
open import cwfs.Pi
open import cwfs.Universe

module reedy.Diagrams {â„“â‚˜á´µ â„“â‚’ â„“â‚˜}
  (I : SimpleSemicategory â„“â‚˜á´µ)
  (I-strictly-oriented : is-strictly-oriented I)
  {C : WildCategory â„“â‚’ â„“â‚˜}
  (cwfstr : CwFStructure C)
  (pistr : PiStructure cwfstr)
  (univstr : UniverseStructure cwfstr)
  where

open SimpleSemicategory I
open import reedy.Cosieves I
open Cosieves-IsStrictlyOriented I-strictly-oriented

open CwFStructure cwfstr renaming (_â—¦_ to _â—¦Ë¢áµ˜áµ‡_)
open PiStructure pistr
open UniverseStructure univstr
open import cwfs.Telescopes cwfstr
open Î â‚œâ‚‘â‚— pistr
open TelIndexedTypes univstr


ğ”» : â„• â†’ Con
Máµ’ : (i h t : â„•) â†’ shape i h t â†’ Tel (ğ”» (1+ h))

-- Convenience definitions ====

M : (i h t : â„•) â†’ shape i h t â†’ Con
M i h t s = close (Máµ’ i h t s)

Máµ’áµ—áµ’áµ— : (i : â„•) â†’ Tel (ğ”» i)
Máµ’áµ—áµ’áµ— O = â€¢
Máµ’áµ—áµ’áµ— (1+ i) = Máµ’ (1+ i) i (hom-size (1+ i) i) (total-shape-1+ i)

Máµ’á¶ áµ˜Ë¡Ë¡ : (i h : â„•) â†’ Tel (ğ”» (1+ h))
Máµ’á¶ áµ˜Ë¡Ë¡ i h = Máµ’ i h full shp
  where
  full = hom-size i h
  shp = full-shape i h

ğ”¸ : (i : â„•) â†’ Ty (ğ”» i)
ğ”¸ i = Î â‚œâ‚‘â‚— (Máµ’áµ—áµ’áµ— i) U

A : (i : â„•) â†’ Ty (ğ”» i âˆ· ğ”¸ i ++â‚œâ‚‘â‚— Máµ’áµ—áµ’áµ— i [ Ï€ (ğ”¸ i) ]â‚œâ‚‘â‚—)
A i = generic[ Máµ’áµ—áµ’áµ— i ]type

M= : âˆ€ i h {t} {s} {t'} {s'} â†’ t == t' â†’ M i h t s == M i h t' s'
M= i h {t} {s} {.t} {s'} idp = ap (M i h t) (shape-path s s')

M=shape : âˆ€ {i h t} s s' â†’ M i h t s == M i h t s'
M=shape {i} {h} {t} s s' = ap (M i h t) (shape-path s s')

-- End convenience definitions ====

ğ”» O = â—†
ğ”» (1+ i) = ğ”» i âˆ· ğ”¸ i

Mâƒ— :
  âˆ€ i h t s {j} (f : hom i j)
  â†’ let cf = count-factors i h t s f
        sh = count-factors-shape i h t s f
    in Sub (M i h t s) (M j h cf sh)

-- Also use this equation
M=â‚ :
  âˆ€ i h t (s : shape i h (1+ t))
  â†’ let prev = prev-shape s
        u = Sâ‰¤-< s
        [t] = #[ t ] i h u
        cf = count-factors i h t prev [t]
        sh = count-factors-shape i h t prev [t]
    in M h h cf sh == close (Máµ’áµ—áµ’áµ— h [ Ï€ (ğ”¸ h) ]â‚œâ‚‘â‚—)

Mâƒ—â—¦ :
  âˆ€ i h t s {j} (f : hom i j) {k} (g : hom j k)
  â†’ let cf = count-factors i h t s f
        sh = count-factors-shape i h t s f -- or abstract over this too?
        p  = count-factors-comp i h t s f g -- and this too?
    in Mâƒ— j h cf sh g â—¦Ë¢áµ˜áµ‡ Mâƒ— i h t s f == idd (M= k h p) â—¦Ë¢áµ˜áµ‡ Mâƒ— i h t s (g â—¦ f)


{-# TERMINATING #-}
Máµ’ i h (1+ t) s =
  Máµ’ i h t prev â€£ A h [ idd eq â—¦Ë¢áµ˜áµ‡ Mâƒ— i h t prev (#[ t ] i h u) ]
  where
  prev = prev-shape s
  u : t < hom-size i h
  u = Sâ‰¤-< s

  c = count-factors i h t prev (#[ t ] i h u)
  cs = count-factors-shape i h t prev (#[ t ] i h u)

  eq : M h h c cs == (ğ”» (1+ h) ++â‚œâ‚‘â‚— Máµ’áµ—áµ’áµ— h [ Ï€ (ğ”¸ h) ]â‚œâ‚‘â‚—)
  eq = M=â‚ i h t s

Máµ’ i (1+ h) O s = Máµ’á¶ áµ˜Ë¡Ë¡ i h [ Ï€ (ğ”¸ (1+ h)) ]â‚œâ‚‘â‚—
Máµ’ i O O s = â€¢

M=â‚ i O t s =
  M O O cf sh =âŸ¨ M= O O {s' = Oâ‰¤ _} p âŸ©
  M O O O (Oâ‰¤ (hom-size O O)) =âŸ¨ idp âŸ©
  close (Máµ’áµ—áµ’áµ— O [ Ï€ (ğ”¸ O) ]â‚œâ‚‘â‚—) =âˆ
  where
  prev = prev-shape s
  u = Sâ‰¤-< s
  [t] = #[ t ] i O u
  cf = count-factors i O t prev [t]
  sh = count-factors-shape i O t prev [t]

  p : cf == O
  p = count-factors-top-level i O t prev [t]

M=â‚ i (1+ h) t s =
  M (1+ h) (1+ h) cf sh =âŸ¨ M= (1+ h) (1+ h) {s' = Oâ‰¤ _} p âŸ©
  M (1+ h) (1+ h) O (Oâ‰¤ _) =âŸ¨ idp âŸ©
  close (Máµ’áµ—áµ’áµ— (1+ h) [ Ï€ (ğ”¸ (1+ h)) ]â‚œâ‚‘â‚—) =âˆ
  where
  prev = prev-shape s
  u = Sâ‰¤-< s
  [t] = #[ t ] i (1+ h) u
  cf = count-factors i (1+ h) t prev [t]
  sh = count-factors-shape i (1+ h) t prev [t]

  p : cf == O
  p = count-factors-top-level i (1+ h) t prev [t]


Mâƒ— i h (1+ O) s {j} f =
  depcase P
    (f âˆ£? #[ O ] i h u)
    yes.sub
    no.sub
  :>
  Sub (M i h 1 s)
      (M j h (count-factors i h 1 s f)
        (count-factors-shape i h 1 s f))
  where
  u : O < hom-size i h
  u = Sâ‰¤-< s

  fâˆ£[O] : Type _
  fâˆ£[O] = f âˆ£ #[ O ] i h u

  P : (d : Dec fâˆ£[O]) â†’ Type _
  P d = Sub (M i h 1 s)
            (M j h (count-factors[ i , h ,1+ O ] u f d)
              (count-factors-shape-aux i h O u f d))

  module yes (w : fâˆ£[O]) where
    prev = prev-shape s
    c = count-factors i h O prev f
    cs = count-factors-shape i h O prev f

    sub : Sub (M i h 1 s) (M j h c _ âˆ· A h [ _ ])
    sub =
      idd (M=shape cs _) â—¦Ë¢áµ˜áµ‡ Mâƒ— i h O prev f â—¦Ë¢áµ˜áµ‡ Ï€ (A h [ _ ])
      ,, {!!}

  module no (w : Â¬ fâˆ£[O]) where
    prev = prev-shape s

    sub : Sub (M i h 1 s) (M j h O _)
    sub = Mâƒ— i h O prev f â—¦Ë¢áµ˜áµ‡ Ï€ (A h [ _ ])

  prev = prev-shape s

Mâƒ— i h (2+ t) s {j} f =
  depcase P
    (f âˆ£? #[ 1+ t ] i h u)
    yes.sub
    no.sub
  :>
  Sub (M i h (2+ t) s)
      (M j h (count-factors i h (2+ t) s f)
        (count-factors-shape i h (2+ t) s f))
  where
  u : 1+ t < hom-size i h
  u = Sâ‰¤-< s

  fâˆ£[t+1] : Type _
  fâˆ£[t+1] = f âˆ£ #[ 1+ t ] i h u

  P : (d : Dec fâˆ£[t+1]) â†’ Type _
  P d = Sub (M i h (2+ t) s)
            (M j h (count-factors[ i , h ,1+ 1+ t ] u f d)
              (count-factors-shape-aux i h (1+ t) u f d))

  module yes (w : fâˆ£[t+1]) where
    prev = prev-shape s
    c = count-factors i h (1+ t) prev f
    cs = count-factors-shape i h (1+ t) prev f

    v : t < hom-size i h
    v = S<-< u

    sub : Sub (M i h (2+ t) s) (M j h c _ âˆ· A h [ _ ])
    sub =
      idd (M=shape cs _) â—¦Ë¢áµ˜áµ‡ Mâƒ— i h (1+ t) prev f â—¦Ë¢áµ˜áµ‡ Ï€ (A h [ _ ])
      ,, {!!}

  module no (w : Â¬ fâˆ£[t+1]) where
    prev = prev-shape s

    sub : Sub (M i h (2+ t) s)
              (M j h (count-factors i h (1+ t) prev f) _)
    sub = Mâƒ— i h (1+ t) prev f â—¦Ë¢áµ˜áµ‡ Ï€ (A h [ _ ])

{- new attempts
--  with f âˆ£ #[ t ] i h (Sâ‰¤-< s)
--     -- | count-factors i h (1+ t) s f in eq
--     -- | count-factors-shape i h (1+ t) s f
--     | Máµ’ j h (count-factors i h (1+ t) s f)
--         (count-factors-shape i h (1+ t) s f)
--     -- | inspect (uncurry $ Máµ’ j h)
--     --           ( count-factors i h (1+ t) s f
--     --           , count-factors-shape i h (1+ t) s f )
-- ... | inl x | Máµ’jh = {!!}
-- ... | inr x | Máµ’jh = {!!}
-}

{- old def
 with f âˆ£ #[ t ] i h (Sâ‰¤-< s)
    | inspect (count-factors i h (1+ t) s) f
    | count-factors i h (1+ t) s f               -- c
    | inspect (count-factors i h (1+ t) s) f
    | count-factors-shape i h (1+ t) s f   -- cs
    | Máµ’ j h (count-factors i h (1+ t) s f)
        (count-factors-shape i h (1+ t) s f)
    | inspect (uncurry $ Máµ’ j h)
        (count-factors i h (1+ t) s f
        , count-factors-shape i h (1+ t) s f)

... | inl (g , e)
    | have p -- : count-factors i h (1+ t) s f ==
             --   1+ (count-factors i h t (prev-shape s) f)
    | c @ .(count-factors i h (1+ t) s f) | have idp
    | cs
    | .(Máµ’ j h (count-factors i h (1+ t) s f) cs) | have idp
      -- Would we be able to pattern match on p if we paired up c and its
      -- inspected equality? More principled: worth manually writing auxiliary
      -- defs to do a proper hand-tailored with-abstraction.
    =
    (idd eq â—¦Ë¢áµ˜áµ‡
      (idd {!!} â—¦Ë¢áµ˜áµ‡ Mâƒ— i h t prev f â—¦Ë¢áµ˜áµ‡ Ï€ (A h [ _ ]) ,, {!!})
    ) :> (Sub (M i h t prev âˆ· A h [ idd (M=â‚ i h t s) â—¦Ë¢áµ˜áµ‡ Mâƒ—iht[t] ]) (M j h c cs))
    where
    prev = prev-shape s
    cf = count-factors i h t prev f

    sh : shape j h (1+ cf)
    sh = transp (shape j h) p cs

    eq : M j h (1+ cf) sh == M j h c cs
    eq = M= j h (! p)

    -- debugging
    u = Sâ‰¤-< s
    Mâƒ—iht[t] = Mâƒ— i h t prev (#[ t ] i h u)
    ----

    Mâƒ—ihtf = Mâƒ— i h t prev f

... | inr no
    | have p -- : count-factors i h (1+ t) s f ==
             --   count-factors i h t (prev-shape s) f
    | c @ .(count-factors i h (1+ t) s f) | have idp
    | cs
    | .(Máµ’ j h (count-factors i h (1+ t) s f) cs) | have idp
    =
    idd eq â—¦Ë¢áµ˜áµ‡ Mâƒ— i h t prev f â—¦Ë¢áµ˜áµ‡ Ï€ (A h [ _ ])
      -- Note (also record this on paper): on paper, don't have this coercion by
      -- (idd _), but in TT we need this because we don't have that
      -- count-factors (i, h, t+1) f reduces to count-factors (i, h, t) f
      -- definitionally. But maybe it can be made so, with more effort?
    where
    prev = prev-shape s
    cf = count-factors i h t prev f
    sh = count-factors-shape i h t prev f

    eq : M j h cf sh == M j h c cs
    eq = M= j h (! p)
-}

Mâƒ— i (1+ h) O s {j} f =
  wkn-sub (Máµ’á¶ áµ˜Ë¡Ë¡ i h) (Máµ’á¶ áµ˜Ë¡Ë¡ j h)
    (idd eq â—¦Ë¢áµ˜áµ‡ Mâƒ— i h fulláµ¢ shpáµ¢ f)
    {!commutation lemma; another component of the definition!}
    (ğ”¸ (1+ h))
  where
  fulláµ¢ = hom-size i h
  shpáµ¢ = full-shape i h

  cf = count-factors i h fulláµ¢ shpáµ¢ f
  sh = count-factors-shape i h fulláµ¢ shpáµ¢ f

  fullâ±¼ = hom-size j h
  shpâ±¼ = full-shape j h

  eq : M j h cf sh == M j h fullâ±¼ shpâ±¼
  eq = M= j h (count-factors-full i h shpáµ¢ f)

Mâƒ— i O O s f = id
Mâƒ—â—¦ i h (1+ t) s f g = {!!}
Mâƒ—â—¦ i (1+ h) O s f g = {!!}
Mâƒ—â—¦ i O O s f {k} g =
  ap (_â—¦Ë¢áµ˜áµ‡ id) (ap (idd âˆ˜ ap (M k O O)) (! $ prop-has-all-paths-idp _))
